
## Physics Problem: Total Energy Dissipated in a Resistor

### Problem:
A voltage signal $v(t)$ is connected across a 5 Ω resistor at $t = 0$. If the voltage is defined by:

$$
v(t) = 2\exp(-3t) + 4\exp(-7t)
$$

What is the total energy dissipated in the resistor?

### Solution:
To find the total energy dissipated in the resistor, we first calculate the instantaneous power dissipated at any time $t$, and then integrate this power over time to find the total energy.

The power dissipated in a resistor is given by:

$$
P(t) = \frac{v^2(t)}{R}
$$

where $v(t)$ is the voltage across the resistor, and $R$ is the resistance. In this case, the resistance $R = 5 \, \Omega$, and the voltage across the resistor is:

$$
v(t) = 2e^{-3t} + 4e^{-7t}
$$

First, compute $v^2(t)$:

$$
v^2(t) = \left( 2e^{-3t} + 4e^{-7t} \right)^2
$$

Expanding this:

$$
v^2(t) = 4e^{-6t} + 16e^{-14t} + 16e^{-10t}
$$

Now, the power $P(t)$ dissipated at any time $t$ is:

$$
P(t) = \frac{v^2(t)}{5} = \frac{4e^{-6t} + 16e^{-14t} + 16e^{-10t}}{5}
$$

Now, to find the total energy dissipated, we integrate the power over time from $t = 0$ to $t = \infty$:

$$
E = \int_0^\infty P(t) \, dt
$$

Substitute the expression for $P(t)$:

$$
E = \int_0^\infty \left( \frac{4e^{-6t}}{5} + \frac{16e^{-14t}}{5} + \frac{16e^{-10t}}{5} \right) dt
$$

We can separate this into three integrals:

$$
E = \frac{4}{5} \int_0^\infty e^{-6t} \, dt + \frac{16}{5} \int_0^\infty e^{-14t} \, dt + \frac{16}{5} \int_0^\infty e^{-10t} \, dt
$$

The integral of $e^{-at}$ is $\frac{1}{a}$, so we compute each term:

$$
\int_0^\infty e^{-6t} \, dt = \frac{1}{6}, \quad \int_0^\infty e^{-14t} \, dt = \frac{1}{14}, \quad \int_0^\infty e^{-10t} \, dt = \frac{1}{10}
$$

Now substitute these values back into the expression for $E$:

$$
E = \frac{4}{5} \cdot \frac{1}{6} + \frac{16}{5} \cdot \frac{1}{14} + \frac{16}{5} \cdot \frac{1}{10}
$$

Simplifying each term:

$$
E = \frac{4}{30} + \frac{16}{70} + \frac{16}{50}
$$

Finding a common denominator:

$$
E = \frac{28}{210} + \frac{48}{210} + \frac{67.2}{210}
$$

$$
E = \frac{143.2}{210}
$$

$$
E \approx 0.682 \, \text{Joules}
$$

Thus, the total energy dissipated in the resistor is approximately $0.682 \text{J}$.

To solve  $\left( 2e^{-3t} + 4e^{-7t} \right)^2$ ￼, we will expand the expression using the distributive property or binomial expansion formula, just like we did for $\left( 2e^{-3t} + 4e^{-7t} \right)^2$ .

Given:

$$￼
\left( 2e^{-3t} + 4e^{-7t} \right)^2 = \left( 2e^{-3t} + 4e^{-7t} \right)\left( 2e^{-3t} + 4e^{-7t} \right)
$$

Now distribute each term:

$$￼
= \left( 2e^{-3t} \right)\left( 2e^{-3t} \right) + \left( 2e^{-3t} \right)\left( 4e^{-7t} \right) + \left( 4e^{-7t} \right)\left( 2e^{-3t} \right) + \left( 4e^{-7t} \right)\left( 4e^{-7t} \right)
$$

Simplify each term:

$$
= 4e^{-6t} + 8e^{-10t} + 8e^{-10t} + 16e^{-14t}
$$
￼

Now combine like terms:

$$
= 4e^{-6t} + 16e^{-10t} + 16e^{-14t}
$$

Thus, the expanded form of   $\left( 2e^{-3t} + 4e^{-7t} \right)^2$  ￼ is:

$$￼
4e^{-6t} + 16e^{-10t} + 16e^{-14t}
$$
